\documentclass[12pt]{article}

\usepackage{amsmath}
\usepackage{amsfonts}
\usepackage[margin=1in]{geometry}
\begin{document}

(Taken from Kloeden, P. and Platen, E. (1995) Numerical Solution of Stochastic Differential Equations. New York: Springer.)

Consider a $d$-dimensional SDE of the form (page 166, 1.24)
%
\begin{equation}
X_\tau = X_\rho + \int_\rho^\tau a(s, X_s) ds + \sum_{j=1}^m \int_\rho^\tau b^j (s, X_s) dW_s^j
\end{equation}
%
and a function 
$$f: \mathbb{R}^{+} \times \mathbb{R}^d \mapsto \mathbb{R}$$
%
From page 182, equation 5.3
%
\begin{equation} \label{eq:ito_taylor}
f(\tau, X_\tau) = \sum_{\alpha \in A} I_\alpha [f_\alpha(\rho, X_\rho)]_{\rho, \tau} + \sum_{\alpha \in B(A)} I_\alpha [f_\alpha (\cdot, X_\cdot)]_{\rho, \tau}
\end{equation}
where 
\begin{itemize}
\item $A \subset M$ is a hierarchical set (page 180)
\item $M$ is the set of multiindices 
\item  $B(A)$ is the remainder set (page 180)
$$B(A) = \left\{ \alpha \in M \ A: -\alpha \in A \right\}$$
\item  $-\alpha$ denotes $a$ with the first entry deleted
\item $\rho$ and $\tau$ are two stopping times
\item $I_\alpha$ denotes the multiple Ito integral (page 168)
\item $f_\alpha$ denotes the Ito coefficient function (page 177)
\end{itemize}


Let 
$$ A = \{ \alpha \in M : l(\alpha) \le 1 \} = \{ (j) : 0 \le j \le m \} \cup \{v \}$$
where $v$ is the empty multiindex.
%
Then
$$B(A) = \{ (j, k) : 0 \le j \le m, 0 \le k \le m \}$$

We can write \eqref{eq:ito_taylor} as
\begin{equation} \label{eq:ito_taylor2}
f( X_\tau) = I_{v} [f_{v} ( X_\rho)]_{\rho, \tau} + \sum_{j=0}^m I_{(j)} [f_{(j)}( X_\rho)]_{\rho, \tau} + \sum_{j=0}^m \sum_{k=0}^m I_{(j,k)} [f_{(j,k)} ( X_\cdot)]_{\rho, \tau}
\end{equation}


We have that (page 169)
\begin{itemize}
\item $I_v [f(\cdot)]_{\rho, \tau} = f(\tau) = \mathcal{O}(1)$
\item $I_{(0)} [f(\cdot)]_{\rho, \tau} = \int_{\rho}^{\tau} f(s) ds = \mathcal{O}(\tau - \rho)$
\item $I_{(j)} [f(\cdot)]_{\rho, \tau} = \int_{\rho}^{\tau} f(s) dW_s^j = \mathcal{O}(\sqrt{\tau - \rho})$, for $j \ge 1$
\item $I_{(0,0)} [f(\cdot)]_{\rho, \tau} = \int_{\rho}^{\tau} \int_{\rho}^{s_2} f(s_1) ds_1 ds_2 = \mathcal{O}((\tau - \rho)^2)$
\item $I_{(j,0)} [f(\cdot)]_{\rho, \tau} = \int_{\rho}^{\tau} \int_{\rho}^{s_2} f(s_1) dW_{s_1}^j ds_2 = \mathcal{O}((\tau - \rho)^{3/2})$, for $j \ge 1$
\item $I_{(0,k)} [f(\cdot)]_{\rho, \tau} = \int_{\rho}^{\tau} \int_{\rho}^{s_2} f(s_1) ds_1 dW_{s_2}^k = \mathcal{O}((\tau - \rho)^{3/2})$, for $k \ge 1$
\item $I_{(j,k)} [f(\cdot)]_{\rho, \tau} = \int_{\rho}^{\tau} \int_{\rho}^{s_2} f(s_1) dW_{s_1}^j dW_{s_2}^k = \mathcal{O}(\tau - \rho)$, for $j, k \ge 1$
\end{itemize}

Then, rewriting \eqref{eq:ito_taylor2} with the terms in order of importance, we have
\begin{equation} \label{eq:ito_taylor_sorted}
\begin{aligned}
f( X_\tau) =& I_{v} [f_{v} ( X_\rho)]_{\rho, \tau}  \\
&+ \sum_{j=1}^d I_{(j)} [f_{(j)}( X_\rho)]_{\rho, \tau} \\ &
+ I_{(0)} [f_{(0)}( X_\rho)]_{\rho, \tau} + \sum_{j=1}^d \sum_{k=1}^d I_{(j,k)} [f_{(j,k)} ( X_\cdot)]_{\rho, \tau} \\
& + \sum_{j=1}^d I_{(j,0)} [f_{(j,0)} ( X_\cdot)]_{\rho, \tau} + \sum_{k=1}^d  I_{(0,k)} [f_{(0,k)} ( X_\cdot)]_{\rho, \tau} \\
& + I_{(0,0)} [f_{(0,0)} ( X_\cdot)]_{\rho, \tau} 
\end{aligned}
\end{equation}

From page 177,
\begin{itemize}
\item $f_v = f$
\item $f_{(j)} = \sum_{k=1}^d b^{k,j} \frac{\partial f}{\partial x^k}$, for $j \ge 1$
\item $f_{(0)} = \frac{\partial f}{\partial t} + \sum_{k=1}^d a^k \frac{\partial f}{\partial x^k} + \frac{1}{2} \sum_{k,l=1}^d \sum_{j=1}^m b^{k,j} b^{l,j} \frac{\partial^2 f}{\partial x^k \partial x^l}$
\item $f_{(j, k)} = \sum_{i=1}^d b^{i,j} \frac{\partial }{\partial x^i} \left( \sum_{l=1}^d b^{l,k} \frac{\partial f}{\partial x^l} \right) $ for $j,k \ge 1$
\item $f_{(j,0)} = \sum_{k=1}^d b^{k,j} \frac{\partial }{\partial x^k} \left( \frac{\partial f}{\partial t} + \sum_{k=1}^d a^k \frac{\partial f}{\partial x^k} + \frac{1}{2} \sum_{k,l=1}^d \sum_{i=1}^m b^{k,i} b^{l,i} \frac{\partial^2 f}{\partial x^k \partial x^l} \right)$
\item $f_{(0, j)} = \left( \frac{\partial}{\partial t} + \sum_{k=1}^d a^k \frac{\partial}{\partial x^k} + \frac{1}{2} \sum_{k,l=1}^d \sum_{i=1}^m b^{k,i} b^{l,i} \frac{\partial^2}{\partial x^k \partial x^l} \right)  \sum_{k=1}^d b^{k,j} \frac{\partial f}{\partial x^k}$ for $j \ge 1$
\item $f_{(0,0)} = \left( \frac{\partial}{\partial t} + \sum_{k=1}^d a^k \frac{\partial}{\partial x^k} + \frac{1}{2} \sum_{k,l=1}^d \sum_{j=1}^m b^{k,j} b^{l,j} \frac{\partial^2}{\partial x^k \partial x^l} \right) $\\ $ \left( \frac{\partial f}{\partial t} + \sum_{k=1}^d a^k \frac{\partial f}{\partial x^k} + \frac{1}{2} \sum_{k,l=1}^d \sum_{j=1}^m b^{k,j} b^{l,j} \frac{\partial^2 f}{\partial x^k \partial x^l} \right)$
\end{itemize}
%
For intrinsic variables, we assume that $b^{j,k} = \delta_{j,k}$, $d=m$, and $f$ does not depend on $t$. 
%
The terms then reduce to
\begin{itemize}
\item $f_v = f$
\item $f_{(j)} = \frac{\partial f}{\partial x^j}$, for $j \ge 1$
\item $f_{(0)} =  \sum_{k=1}^d a^k \frac{\partial f}{\partial x^k} + \frac{1}{2} \sum_{j=1}^d \frac{\partial^2 f}{\partial {x^j}^2}$
\item $f_{(j, k)} = \frac{\partial }{\partial x^j} \left( \frac{\partial f}{\partial x^k} \right) = \frac{\partial^2 f}{\partial x^j \partial x^k}$ for $j,k \ge 1$
\item $f_{(j,0)} = \frac{\partial }{\partial x^j} \left( \sum_{k=1}^d a^k \frac{\partial f}{\partial x^k} + \frac{1}{2} \sum_{k=1}^d \frac{\partial^2 f}{\partial x^k \partial x^k} \right)$ \\
$ =  \sum_{k=1}^d a^k \frac{\partial^2 f}{\partial x^j \partial x^k} + \frac{1}{2} \sum_{k=1}^d \frac{\partial^3 f}{\partial x^j \partial {x^k}^2}$ 
\item $f_{(0, j)} = \left( \sum_{k=1}^d a^k \frac{\partial}{\partial x^k} + \frac{1}{2} \sum_{k=1}^d  \frac{\partial^2}{\partial x^k \partial x^k} \right) \frac{\partial f}{\partial x^j}$ \\
$= \sum_{k=1}^d a^k \frac{\partial^ f}{\partial x^k \partial x^j} + \frac{1}{2} \sum_{k=1}^d  \frac{\partial^3 f}{\partial {x^k}^2 \partial x^j}$ for $j \ge 1$
\item $f_{(0,0)} = \left( \sum_{j=1}^d a^j \frac{\partial}{\partial x^j} + \frac{1}{2} \sum_{j=1}^d  \frac{\partial^2}{\partial x^j \partial x^j} \right) \left( \sum_{k=1}^d a^k \frac{\partial f}{\partial x^k} + \frac{1}{2} \sum_{k=1}^d \frac{\partial^2 f}{\partial x^k \partial x^k} \right)$ \\
$= \sum_{j=1}^d \sum_{k=1}^d \left[ a^j \frac{\partial}{\partial x^j}\left( a^k \frac{\partial f}{\partial x^k} \right) + \frac{1}{2} \frac{\partial^2}{\partial {x^j}^2} \left( a^k \frac{\partial f}{\partial x^k} \right) + \frac{1}{2} a^j \frac{\partial^3 f}{\partial x^j \partial {x^k}^2} + \frac{1}{4} \frac{\partial^4 f}{\partial {x^j}^2 \partial {x^k}^2} \right]$
\end{itemize}

Then, substituting into \eqref{eq:ito_taylor_sorted}, we obtain
\begin{equation}
\begin{aligned}
f( X_\tau) = & f( X_\rho) \\
&+ \sum_{j=1}^d \left. \frac{\partial f}{\partial x^j} \right|_{X_\rho}  \int_{\rho}^{\tau}  dW_s^j \\ &
+  \left. \left( \sum_{k=1}^d a^k \frac{\partial f}{\partial x^k} + \frac{1}{2} \sum_{j=1}^d \frac{\partial^2 f}{\partial {x^j}^2} \right) \right|_{X_\rho} \int_{\rho}^{\tau} ds + \sum_{j=1}^m \sum_{k=1}^m \int_{\rho}^{\tau} \int_{\rho}^{s_2} \frac{\partial^2 f}{\partial x^j \partial x^k} dW_{s_1}^j dW_{s_2}^k \\
& + \sum_{j=1}^d  \int_{\rho}^{\tau} \int_{\rho}^{s_2} \left( \sum_{k=1}^d a^k \frac{\partial^2 f}{\partial x^j \partial x^k} + \frac{1}{2} \sum_{k=1}^d \frac{\partial^3 f}{\partial x^j \partial {x^k}^2} \right) dW_{s_1}^j ds_2 \\
& + \sum_{j=1}^d  \int_{\rho}^{\tau} \int_{\rho}^{s_2} \left( \sum_{k=1}^d a^k \frac{\partial^ f}{\partial x^k \partial x^j} + \frac{1}{2} \sum_{k=1}^d  \frac{\partial^3 f}{\partial {x^k}^2 \partial x^j} \right) ds_1 dW_{s_2}^j  \\
& + \int_{\rho}^{\tau} \int_{\rho}^{s_2} \left( \sum_{j=1}^d \sum_{k=1}^d \left[ a^j \frac{\partial}{\partial x^j}\left( a^k \frac{\partial f}{\partial x^k} \right) + \frac{1}{2} \frac{\partial^2}{\partial {x^j}^2} \left( a^k \frac{\partial f}{\partial x^k} \right) + \frac{1}{2} a^j \frac{\partial^3 f}{\partial x^j \partial {x^k}^2} + \frac{1}{4} \frac{\partial^4 f}{\partial {x^j}^2 \partial {x^k}^2} \right] \right)  ds_1 ds_2
\end{aligned}
\end{equation}

There are two terms that are $\mathcal{O}(\tau - \rho)$:
\begin{itemize}
\item $\left. \left( \sum_{k=1}^d a^k \frac{\partial f}{\partial x^k} + \frac{1}{2} \sum_{j=1}^d \frac{\partial^2 f}{\partial {x^j}^2} \right) \right|_{X_\rho} \int_{\rho}^{\tau} ds $
\item $ \sum_{j=1}^m \sum_{k=1}^m \int_{\rho}^{\tau} \int_{\rho}^{s_2} \frac{\partial^2 f}{\partial x^j \partial x^k} dW_{s_1}^j dW_{s_2}^k $
\end{itemize}

\end{document}