\documentclass[12pt]{article}

\usepackage{amsmath}
\usepackage{amsfonts}
\usepackage[margin=1in]{geometry}
\begin{document}

(Taken from Kloeden, P. and Platen, E. (1995) Numerical Solution of Stochastic Differential Equations. New York: Springer.)

Consider a $n$-dimensional SDE of the form (page 166, 1.24)
%
\begin{equation}
X_\tau = X_\rho + \int_\rho^\tau a(s, X_s) ds + \sum_{j=1}^n \int_\rho^\tau b^j (s, X_s) dW_s^j
\end{equation}
(note: for NIV/multiscale SDEs, we will assume the dimension of the Brownian motion will be the same as the dimension of the SDE)
%
and a function 
$$f: \mathbb{R}^{+} \times \mathbb{R}^n \mapsto \mathbb{R}$$
%
From page 182, equation 5.3
%
\begin{equation} \label{eq:ito_taylor}
f(\tau, X_\tau) = \sum_{\alpha \in A} I_\alpha [f_\alpha(\rho, X_\rho)]_{\rho, \tau} + \sum_{\alpha \in B(A)} I_\alpha [f_\alpha (\cdot, X_\cdot)]_{\rho, \tau}
\end{equation}
where 
\begin{itemize}
\item $A \subset M$ is a hierarchical set (page 180)
\item $M$ is the set of multiindices 
\item  $B(A)$ is the remainder set (page 180)
$$B(A) = \left\{ \alpha \in M \ A: -\alpha \in A \right\}$$
\item  $-\alpha$ denotes $a$ with the first entry deleted
\item $\rho$ and $\tau$ are two stopping times
\item $I_\alpha$ denotes the multiple Ito integral (page 168)
\item $f_\alpha$ denotes the Ito coefficient function (page 177)
\end{itemize}


Let 
$$ A = \{ \alpha \in M : l(\alpha) \le 1 \} = \{ (j) : 0 \le j \le n \} \cup \{v \}$$
where $v$ is the empty multiindex.
%
Then
$$B(A) = \{ (j, k) : 0 \le j \le n, 0 \le k \le n \}$$

We can write \eqref{eq:ito_taylor} as
\begin{equation} \label{eq:ito_taylor2}
f( X_\tau) = I_{v} [f_{v} ( X_\rho)]_{\rho, \tau} + \sum_{j=0}^n I_{(j)} [f_{(j)}( X_\rho)]_{\rho, \tau} + \sum_{j=0}^n \sum_{k=0}^n I_{(j,k)} [f_{(j,k)} ( X_\cdot)]_{\rho, \tau}
\end{equation}


We have that (page 169)
\begin{itemize}
\item $I_v [f(\cdot)]_{\rho, \tau} = f(\tau) = \mathcal{O}(1)$
\item $I_{(0)} [f(\cdot)]_{\rho, \tau} = \int_{\rho}^{\tau} f(s) ds = \mathcal{O}(\tau - \rho)$
\item $I_{(j)} [f(\cdot)]_{\rho, \tau} = \int_{\rho}^{\tau} f(s) dW_s^j = \mathcal{O}(\sqrt{\tau - \rho})$, for $j \ge 1$
\item $I_{(0,0)} [f(\cdot)]_{\rho, \tau} = \int_{\rho}^{\tau} \int_{\rho}^{s_2} f(s_1) ds_1 ds_2 = \mathcal{O}((\tau - \rho)^2)$
\item $I_{(j,0)} [f(\cdot)]_{\rho, \tau} = \int_{\rho}^{\tau} \int_{\rho}^{s_2} f(s_1) dW_{s_1}^j ds_2 = \mathcal{O}((\tau - \rho)^{3/2})$, for $j \ge 1$
\item $I_{(0,k)} [f(\cdot)]_{\rho, \tau} = \int_{\rho}^{\tau} \int_{\rho}^{s_2} f(s_1) ds_1 dW_{s_2}^k = \mathcal{O}((\tau - \rho)^{3/2})$, for $k \ge 1$
\item $I_{(j,k)} [f(\cdot)]_{\rho, \tau} = \int_{\rho}^{\tau} \int_{\rho}^{s_2} f(s_1) dW_{s_1}^j dW_{s_2}^k = \mathcal{O}(\tau - \rho)$, for $j, k \ge 1$
\end{itemize}

Then, rewriting \eqref{eq:ito_taylor2} with the terms in order of importance, we have
\begin{equation} \label{eq:ito_taylor_sorted}
\begin{aligned}
f( X_\tau) =& I_{v} [f_{v} ( X_\rho)]_{\rho, \tau}  \\
&+ \sum_{j=1}^d I_{(j)} [f_{(j)}( X_\rho)]_{\rho, \tau} \\ &
+ I_{(0)} [f_{(0)}( X_\rho)]_{\rho, \tau} + \sum_{j=1}^d \sum_{k=1}^d I_{(j,k)} [f_{(j,k)} ( X_\cdot)]_{\rho, \tau} \\
& + \sum_{j=1}^d I_{(j,0)} [f_{(j,0)} ( X_\cdot)]_{\rho, \tau} + \sum_{k=1}^d  I_{(0,k)} [f_{(0,k)} ( X_\cdot)]_{\rho, \tau} \\
& + I_{(0,0)} [f_{(0,0)} ( X_\cdot)]_{\rho, \tau} 
\end{aligned}
\end{equation}

From page 177,
\begin{itemize}
\item $f_v = f$
\item $f_{(j)} = \sum_{k=1}^n b^{k,j} \frac{\partial f}{\partial x^k}$, for $j \ge 1$
\item $f_{(0)} = \frac{\partial f}{\partial t} + \sum_{k=1}^n a^k \frac{\partial f}{\partial x^k} + \frac{1}{2} \sum_{k,l=1}^n \sum_{j=1}^n b^{k,j} b^{l,j} \frac{\partial^2 f}{\partial x^k \partial x^l}$
\item $f_{(j, k)} = \sum_{i=1}^n b^{i,j} \frac{\partial }{\partial x^i} \left( \sum_{l=1}^n b^{l,k} \frac{\partial f}{\partial x^l} \right) $ for $j,k \ge 1$
\item $f_{(j,0)} = \sum_{k=1}^n b^{k,j} \frac{\partial }{\partial x^k} \left( \frac{\partial f}{\partial t} + \sum_{k=1}^n a^k \frac{\partial f}{\partial x^k} + \frac{1}{2} \sum_{k,l=1}^n \sum_{i=1}^n b^{k,i} b^{l,i} \frac{\partial^2 f}{\partial x^k \partial x^l} \right)$
\item $f_{(0, j)} = \left( \frac{\partial}{\partial t} + \sum_{k=1}^n a^k \frac{\partial}{\partial x^k} + \frac{1}{2} \sum_{k,l=1}^n \sum_{i=1}^n b^{k,i} b^{l,i} \frac{\partial^2}{\partial x^k \partial x^l} \right)  \sum_{k=1}^n b^{k,j} \frac{\partial f}{\partial x^k}$ for $j \ge 1$
\item $f_{(0,0)} = \left( \frac{\partial}{\partial t} + \sum_{k=1}^n a^k \frac{\partial}{\partial x^k} + \frac{1}{2} \sum_{k,l=1}^n \sum_{j=1}^n b^{k,j} b^{l,j} \frac{\partial^2}{\partial x^k \partial x^l} \right) $\\ $ \left( \frac{\partial f}{\partial t} + \sum_{k=1}^n a^k \frac{\partial f}{\partial x^k} + \frac{1}{2} \sum_{k,l=1}^n \sum_{j=1}^n b^{k,j} b^{l,j} \frac{\partial^2 f}{\partial x^k \partial x^l} \right)$
\end{itemize}

For intrinsic variables, we assume an equation of the following form 
\begin{equation} \label{eq:general_SDE}
\begin{aligned}
dx_i &= a_i(x_1, \dots, x_n) dt + dW_i, \: 1 \le i \le m \\
dx_i &= -\frac{a_i(x_1, \dots, x_n)}{\epsilon} dt + \frac{1}{\sqrt{\epsilon}} dW_i , \: m+1 \le i \le n
\end{aligned}
\end{equation}
where $W_i$ are independent Brownian motions, and $\epsilon \ll 1$.
%
We also assume that $\frac{\partial f}{\partial t} = 0$. 
%
Therefore,
\begin{equation}
\begin{aligned}
a^i \mapsto a_i, \: & 1 \le i \le m \\
a^i \mapsto \frac{a_i}{\epsilon}, \: & m+1 \le i \le n \\
b^{i,j} \mapsto \delta_{ij}, \: & 1 \le i \le m \\
b^{i,j} \mapsto \frac{\delta_{ij}}{\sqrt{\epsilon}}, \: & m+1 \le i \le n 
\end{aligned}
\end{equation}
%
and so the terms reduce to
%
\begin{itemize}
\item $f_v = f$
%
\item $f_{(j)} = \frac{\partial f}{\partial x_j}$, for $1 \le j \le m$
\item $f_{(j)} = \frac{1}{\sqrt{\epsilon}} \frac{\partial f}{\partial x_j}$, for $m+1 \le j \le n$
%
\item $f_{(0)} = \sum_{k=1}^m a_k \frac{\partial f}{\partial x_k} 
+ \frac{1}{\epsilon} \sum_{k=m+1}^n a_k \frac{\partial f}{\partial x_k} 
+ \frac{1}{2} \sum_{k=1}^m \frac{\partial^2 f}{\partial x_k^2}
+ \frac{1}{2 \epsilon} \sum_{k=m+1}^n \frac{\partial^2 f}{\partial x_k^2}$
%
\item $f_{(j, k)} =  \frac{\partial^2 f}{\partial x_j \partial x_k}  $ for $1 \le j,k \le m$
\item $f_{(j, k)} =  \frac{1}{\sqrt{\epsilon}} \frac{\partial^2 f}{\partial x_j \partial x_k} $ for $m+1 \le j \le n$, $1 \le k \le m$
\item $f_{(j, k)} =  \frac{1}{\sqrt{\epsilon}} \frac{\partial^2 f}{\partial x_j \partial x_k} $ for $1 \le j \le m$, $ m+1 \le k \le n$
\item $f_{(j, k)} =  \frac{1}{\epsilon} \frac{\partial^2 f}{\partial x_j \partial x_k} $ for $m+1 \le j,k \le n$
%
\item $f_{(j,0)} = \sum_{k=1}^m \frac{\partial }{\partial x_j} \left( a_k \frac{\partial f}{\partial x_k} \right) + \frac{1}{\epsilon} \sum_{k=m+1}^m \frac{\partial }{\partial x_j} \left( a_k \frac{\partial f}{\partial x_k} \right) + \frac{1}{2} \sum_{k=1}^m \frac{\partial^3 f}{\partial x_j \partial x_k^2} + \frac{1}{2 \epsilon} \sum_{k=m+1}^n \frac{\partial^3 f}{\partial x_j \partial x_k^2} $ for $1 \le j \le m$
\item $f_{(j,0)} = \frac{1}{\sqrt{\epsilon}} \sum_{k=1}^m \frac{\partial }{\partial x_j} \left( a_k \frac{\partial f}{\partial x_k} \right) + \frac{1}{\epsilon^{3/2}} \sum_{k=m+1}^m \frac{\partial }{\partial x_j} \left( a_k \frac{\partial f}{\partial x_k} \right) + \frac{1}{2 \sqrt{\epsilon}} \sum_{k=1}^m \frac{\partial^3 f}{\partial x_j \partial x_k^2} + \frac{1}{2 \epsilon^{3/2}} \sum_{k=m+1}^n \frac{\partial^3 f}{\partial x_j \partial x_k^2} $ for $m+1 \le j \le n$
%
\item $f_{(0, j)} = \sum_{k=1}^m a_k \frac{\partial^2 f}{\partial x_k \partial x_j} 
+ \frac{1}{\epsilon} \sum_{k=m+1}^n a_k \frac{\partial^2 f}{\partial x_k \partial x_j} 
 + \frac{1}{2} \sum_{k=1}^m \frac{\partial^3 f}{\partial x_k^2 \partial x_j} 
 +\frac{1}{2 \epsilon} \sum_{k=m+1}^n \frac{\partial^3 f}{\partial x_k^2 \partial x_j}$ for $1 \le j \le m$
\item $f_{(0, j)} = \frac{1}{\sqrt{\epsilon}}  \left(\sum_{k=1}^m a_k \frac{\partial^2 f}{\partial x_k \partial x_j} 
+ \frac{1}{\epsilon} \sum_{k=m+1}^n a_k \frac{\partial^2 f}{\partial x_k \partial x_j} 
 + \frac{1}{2} \sum_{k=1}^m \frac{\partial^3 f}{\partial x_k^2 \partial x_j} 
 +\frac{1}{2 \epsilon} \sum_{k=m+1}^n \frac{\partial^3 f}{\partial x_k^2 \partial x_j} \right)$ for $m+1 \le j \le n$
%
\item $f_{(0,0)} = \left(\sum_{k=1}^m a_k \frac{\partial}{\partial x_k} 
+ \frac{1}{\epsilon} \sum_{k=m+1}^n a_k \frac{\partial}{\partial x_k} 
+ \frac{1}{2} \sum_{k=1}^m \frac{\partial^2}{\partial x_k^2} 
+ \frac{1}{2 \epsilon} \sum_{k=m+1}^n \frac{\partial^2}{\partial x_k^2} \right) $\\
$ \left(\sum_{k=1}^m a_k \frac{\partial f}{\partial x_k} 
+ \frac{1}{\epsilon} \sum_{k=m+1}^n a_k \frac{\partial f}{\partial x_k} 
+ \frac{1}{2} \sum_{k=1}^m \frac{\partial^2 f}{\partial x_k^2} 
+ \frac{1}{2 \epsilon} \sum_{k=m+1}^n \frac{\partial^2 f}{\partial x_k^2} \right)$ \\
$= \left(\sum_{k=1}^m \left( a_k \frac{\partial}{\partial x_k} + \frac{1}{2} \frac{\partial^2}{\partial x_k^2} \right) 
+ \frac{1}{\epsilon} \sum_{k=m+1}^n \left( a_k \frac{\partial}{\partial x_k} + \frac{1}{2} \frac{\partial^2}{\partial x_k^2}  \right) \right) $\\
$ \left(\sum_{k=1}^m \left( a_k \frac{\partial f}{\partial x_k} + \frac{1}{2} \frac{\partial^2 f}{\partial x_k^2} \right) 
+ \frac{1}{\epsilon} \sum_{k=m+1}^n \left( a_k \frac{\partial f}{\partial x_k} + \frac{1}{2} \frac{\partial^2 f}{\partial x_k^2}  \right) \right) $ \\
$ = \sum_{j=1}^m \sum_{k=1}^m \left[ a_j \frac{\partial}{\partial x_j} \left( a_k \frac{\partial f}{\partial x_k} \right) + \frac{a_j}{2} \frac{\partial}{\partial x_j} \left( \frac{\partial^2 f}{\partial x_k^2} \right) + \frac{1}{2} \frac{\partial^2}{\partial x_j^2} \left( a_k \frac{\partial f}{\partial x_k} \right) + \frac{1}{4} \frac{\partial^4 f}{\partial x_j^2 \partial x_k^2} \right] $\\
$+ \frac{1}{\epsilon} \sum_{j=m+1}^n \sum_{k=1}^m \left[ a_j \frac{\partial}{\partial x_j} \left( a_k \frac{\partial f}{\partial x_k} \right) + \frac{a_j}{2} \frac{\partial}{\partial x_j} \left( \frac{\partial^2 f}{\partial x_k^2} \right) + \frac{1}{2} \frac{\partial^2}{\partial x_j^2} \left( a_k \frac{\partial f}{\partial x_k} \right) + \frac{1}{4} \frac{\partial^4 f}{\partial x_j^2 \partial x_k^2} \right] $\\
$+ \frac{1}{\epsilon} \sum_{j=1}^m \sum_{k= m+1}^n \left[ a_j \frac{\partial}{\partial x_j} \left( a_k \frac{\partial f}{\partial x_k} \right) + \frac{a_j}{2} \frac{\partial}{\partial x_j} \left( \frac{\partial^2 f}{\partial x_k^2} \right) + \frac{1}{2} \frac{\partial^2}{\partial x_j^2} \left( a_k \frac{\partial f}{\partial x_k} \right) + \frac{1}{4} \frac{\partial^4 f}{\partial x_j^2 \partial x_k^2} \right] $\\
$+ \frac{1}{\epsilon^2} \sum_{j=m+1}^n \sum_{k=m+1}^n \left[ a_j \frac{\partial}{\partial x_j} \left( a_k \frac{\partial f}{\partial x_k} \right) + \frac{a_j}{2} \frac{\partial}{\partial x_j} \left( \frac{\partial^2 f}{\partial x_k^2} \right) + \frac{1}{2} \frac{\partial^2}{\partial x_j^2} \left( a_k \frac{\partial f}{\partial x_k} \right) + \frac{1}{4} \frac{\partial^4 f}{\partial x_j^2 \partial x_k^2} \right]  $
\end{itemize}

Therefore, 
\begin{equation} 
\begin{aligned}
f( X_\tau) =& f(X_\rho) \\
& + \sum_{j=1}^n f_{(j)} (X_\rho) \int_\rho^\tau dW_s^j 
  + f_{(0)} (X_\rho) \int_\rho^\tau ds \\
& + \sum_{j=1}^n \sum_{k=1}^n \int_\rho^\tau \int_\rho^{s_2} f_{(j,k)} (s_1) dW_{s_1}^j dW_{s_2}^k \\
& + \sum_{j=1}^n \int_\rho^\tau \int_\rho^{s_2} f_{(j,0)} (s_1) dW_{s_1}^j ds_2 \\
& + \sum_{k=1}^n \int_\rho^\tau \int_\rho^{s_2} f_{(0,k)} (s_1) ds_1 dW_{s_2}^k \\
& + \int_\rho^\tau \int_\rho^{s_2} f_{(0,0)} (s_1) ds_1 ds_2 
\end{aligned}
\end{equation}


We are interested in the covariance
\begin{equation}
\mathbb{E}\left[ f_1(X_\tau) f_2(X_\tau) \right] - \mathbb{E}\left[ f_1(X_\tau) \right] \mathbb{E}\left[ f_2(X_\tau) \right]  
\end{equation}

The ``real term'' that we are interested in will be $\mathcal{O} (\tau - \rho)$, since it comes from the $dW_s dW_s$ term.
%
Therefore, we will retain terms up to $\mathcal{O} ((\tau - \rho)^{3/2})$.
%
We have
\begin{equation}
\begin{aligned}
&f_1(X_\tau) f_2(X_\tau) = \\
 f_1(X_\rho) & \left( f_2(X_\rho) 
 + \sum_{j=1}^n f_{2(j)} (X_\rho) \int_\rho^\tau dW_s^j 
  + f_{2(0)} (X_\rho) \int_\rho^\tau ds \right. \\
& + \sum_{j=1}^n \sum_{k=1}^n \int_\rho^\tau \int_\rho^{s_2} f_{2(j,k)} (s_1) dW_{s_1}^j dW_{s_2}^k 
 + \sum_{j=1}^n \int_\rho^\tau \int_\rho^{s_2} f_{2(j,0)} (s_1) dW_{s_1}^j ds_2 \\
& \left. + \sum_{k=1}^n \int_\rho^\tau \int_\rho^{s_2} f_{2(0,k)} (s_1) ds_1 dW_{s_2}^k  \right) \\
+ \sum_{j=1}^n f_{1(j)} (X_\rho) \int_\rho^\tau dW_s^j  & \left( f_2(X_\rho) 
 + \sum_{j=1}^n f_{2(j)} (X_\rho) \int_\rho^\tau dW_s^j 
  + f_{2(0)} (X_\rho) \int_\rho^\tau ds \right. \\
& \left. + \sum_{j=1}^n \sum_{k=1}^n \int_\rho^\tau \int_\rho^{s_2} f_{2(j,k)} (s_1) dW_{s_1}^j dW_{s_2}^k  \right) \\
+ f_{1(0)} (X_\rho) \int_\rho^\tau ds & \left( f_2(X_\rho) 
 + \sum_{j=1}^n f_{2(j)} (X_\rho) \int_\rho^\tau dW_s^j  \right) \\
+ \sum_{j=1}^n \sum_{k=1}^n \int_\rho^\tau \int_\rho^{s_2} f_{1(j,k)} (s_1) dW_{s_1}^j dW_{s_2}^k 
& \left( f_2(X_\rho) + \sum_{j=1}^n f_{2(j)} (X_\rho) \int_\rho^\tau dW_s^j \right)\\
& + \sum_{j=1}^n \int_\rho^\tau \int_\rho^{s_2} f_{1(j,0)} (s_1) dW_{s_1}^j ds_2 f_2(X_\rho)\\
& + \sum_{k=1}^n \int_\rho^\tau \int_\rho^{s_2} f_{1(0,k)} (s_1) ds_1 dW_{s_2}^k f_2(X_\rho) \\
&+ \mathcal{O} ((\tau - \rho)^2 ) 
\end{aligned}
\end{equation}

Therefore, we have
\begin{equation}
\begin{aligned}
&\mathbb{E} \left[ f_1(X_\tau) f_2(X_\tau) \right] = \\
 f_1(X_\rho) & \left( f_2(X_\rho) 
  + f_{2(0)} (X_\rho) (\tau - \rho) 
  + \sum_{j=1}^n \sum_{k=1}^n \mathbb{E} \left[ \int_\rho^\tau \int_\rho^{s_2} f_{2(j,k)} (s_1) dW_{s_1}^j dW_{s_2}^k \right] \right. \\
& \left. + \sum_{j=1}^n \mathbb{E} \left[ \int_\rho^\tau \int_\rho^{s_2} f_{2(j,0)} (s_1) dW_{s_1}^j ds_2 \right] 
+ \sum_{k=1}^n \mathbb{E} \left[ \int_\rho^\tau \int_\rho^{s_2} f_{2(0,k)} (s_1) ds_1 dW_{s_2}^k \right]  \right) \\
& +  \sum_{i=1}^n \sum_{j=1}^n f_{1(i)} (X_\rho) f_{2(j)} (X_\rho) \mathbb{E} \left[ \left( \int_\rho^\tau dW_s^i \right) \left( \int_\rho^\tau dW_s^j \right) \right] \\
& + \sum_{i=1}^n \sum_{j=1}^n \sum_{k=1}^n f_{1(i)} (X_\rho) \mathbb{E} \left[ \left( \int_\rho^\tau dW_s^i  \right) \left( \int_\rho^\tau \int_\rho^{s_2} f_{2(j,k)} (s_1) dW_{s_1}^j dW_{s_2}^k  \right) \right] \\
& + f_{1(0)} (X_\rho) f_2(X_\rho) (\tau - \rho) \\
&+ \sum_{j=1}^n \sum_{k=1}^n f_2(X_\rho) \mathbb{E} \left[ \int_\rho^\tau \int_\rho^{s_2} f_{1(j,k)} (s_1) dW_{s_1}^j dW_{s_2}^k \right] \\
& + \sum_{i=1}^n \sum_{j=1}^n \sum_{k=1}^n  f_{2(i)} (X_\rho)  \mathbb{E} \left[ \left( \int_\rho^\tau dW_s^i \right)  \left( \int_\rho^\tau \int_\rho^{s_2} f_{1(j,k)} (s_1) dW_{s_1}^j dW_{s_2}^k \right) \right] \\
& + f_2(X_\rho) \sum_{j=1}^n \mathbb{E} \left[  \int_\rho^\tau \int_\rho^{s_2} f_{1(j,0)} (s_1) dW_{s_1}^j ds_2 \right] \\
& + f_2(X_\rho) \sum_{k=1}^n \mathbb{E} \left[ \int_\rho^\tau \int_\rho^{s_2} f_{1(0,k)} (s_1) ds_1 dW_{s_2}^k \right] \\
&+ \mathcal{O} ((\tau - \rho)^2 ) 
\end{aligned}
\end{equation}
%
and
\begin{equation}
\begin{aligned}
\mathbb{E} [f(X_\tau)] =&  f(X_\rho) \\
& + f_{(0)} (X_\rho) (\tau - \rho) \\
& + \sum_{j=1}^n \sum_{k=1}^n \mathbb{E} \left[ \int_\rho^\tau \int_\rho^{s_2} f_{(j,k)} (s_1) dW_{s_1}^j dW_{s_2}^k  \right]\\
& + \sum_{j=1}^n \mathbb{E} \left[ \int_\rho^\tau \int_\rho^{s_2} f_{(j,0)} (s_1) dW_{s_1}^j ds_2 \right] \\
& + \sum_{k=1}^n \mathbb{E} \left[ \int_\rho^\tau \int_\rho^{s_2} f_{(0,k)} (s_1) ds_1 dW_{s_2}^k \right] \\
& + \int_\rho^\tau \int_\rho^{s_2} f_{(0,0)} (s_1) ds_1 ds_2 
\end{aligned}
\end{equation}

\begin{equation}
\begin{aligned}
& \mathbb{E}[f_1(X_\tau)]\mathbb{E}[f_2(X_\tau)] = \\
f_1(X_\rho) 
& \left(  f_2(X_\rho) 
 + f_{2(0)} (X_\rho) (\tau - \rho) 
 + \sum_{j=1}^n \sum_{k=1}^n \mathbb{E} \left[ \int_\rho^\tau \int_\rho^{s_2} f_{2(j,k)} (s_1) dW_{s_1}^j dW_{s_2}^k  \right] \right. \\
& \left. + \sum_{j=1}^n \mathbb{E} \left[ \int_\rho^\tau \int_\rho^{s_2} f_{2(j,0)} (s_1) dW_{s_1}^j ds_2 \right] 
 + \sum_{k=1}^n \mathbb{E} \left[ \int_\rho^\tau \int_\rho^{s_2} f_{2(0,k)} (s_1) ds_1 dW_{s_2}^k \right]\right) \\
& + f_{1(0)} (X_\rho) f_2(X_\rho) (\tau - \rho) \\
& + f_2(X_\rho) \left(  \sum_{j=1}^n \sum_{k=1}^n \mathbb{E} \left[ \int_\rho^\tau \int_\rho^{s_2} f_{1(j,k)} (s_1) dW_{s_1}^j dW_{s_2}^k  \right] \right) \\
& + f_2(X_\rho) \left(  \sum_{j=1}^n \mathbb{E} \left[ \int_\rho^\tau \int_\rho^{s_2} f_{1(j,0)} (s_1) dW_{s_1}^j ds_2 \right] 
 + \sum_{k=1}^n \mathbb{E} \left[ \int_\rho^\tau \int_\rho^{s_2} f_{1(0,k)} (s_1) ds_1 dW_{s_2}^k \right]\right) \\
& + \mathcal{O} ((\tau - \rho)^2)
\end{aligned}
\end{equation}

And therefore, the covariance is given by
\begin{equation}
\begin{aligned}
&\mathbb{E} \left[ f_1(X_\tau) f_2(X_\tau) \right] - \mathbb{E}[f_1(X_\tau)]\mathbb{E}[f_2(X_\tau)] = \\
& \sum_{i=1}^n \sum_{j=1}^n f_{1(i)} (X_\rho) f_{2(j)} (X_\rho) \mathbb{E} \left[ \left( \int_\rho^\tau dW_s^i \right) \left( \int_\rho^\tau dW_s^j \right) \right] \\
& + \sum_{i=1}^n \sum_{j=1}^n \sum_{k=1}^n f_{1(i)} (X_\rho) \mathbb{E} \left[ \left( \int_\rho^\tau dW_s^i  \right) \left( \int_\rho^\tau \int_\rho^{s_2} f_{2(j,k)} (s_1) dW_{s_1}^j dW_{s_2}^k  \right) \right] \\
& + \sum_{i=1}^n \sum_{j=1}^n \sum_{k=1}^n  f_{2(i)} (X_\rho)  \mathbb{E} \left[ \left( \int_\rho^\tau dW_s^i \right)  \left( \int_\rho^\tau \int_\rho^{s_2} f_{1(j,k)} (s_1) dW_{s_1}^j dW_{s_2}^k \right) \right] \\
&+ \mathcal{O} ((\tau - \rho)^2 ) 
\end{aligned}
\end{equation}

\section{No nonlinearities}

However, we will also consider a second case, where $f$ only defines a rescaling.
%
Let $\frac{\partial f}{\partial x_j} = c_j$, where $c_j$ is a constant.
%
In this case, the higher order derivatives of $f$ are 0, and we have
%
\begin{itemize}
\item $f_v = f$
%
\item $f_{(j)} = c_j$, for $1 \le j \le m$
\item $f_{(j)} = \frac{1}{\sqrt{\epsilon}} c_j$, for $m+1 \le j \le n$
%
\item $f_{(0)} = \sum_{k=1}^m a_k c_k
+ \frac{1}{\epsilon} \sum_{k=m+1}^n a_k c_k$
%
\item $f_{(j, k)} =  0  $ for $1 \le j,k \le n$
%
\item $f_{(j,0)} = \sum_{k=1}^m \frac{\partial a_k}{\partial x_j} c_k  + \frac{1}{\epsilon} \sum_{k=m+1}^m \frac{\partial a_k }{\partial x_j} c_k $ for $1 \le j \le m$
\item $f_{(j,0)} = \frac{1}{\sqrt{\epsilon}} \sum_{k=1}^m \frac{\partial a_k }{\partial x_j} c_k  + \frac{1}{\epsilon^{3/2}} \sum_{k=m+1}^m \frac{\partial a_k}{\partial x_j} c_k$ for $m+1 \le j \le n$
%
\item $f_{(0, j)} =0 $ for $1 \le j \le n$
%
\item $f_{(0,0)}  = \sum_{j=1}^m \sum_{k=1}^m \left[ a_j \frac{\partial a_k}{\partial x_j} c_k + \frac{1}{2} \frac{\partial^2 a_k}{\partial x_j^2} c_k \right] 
+ \frac{1}{\epsilon} \sum_{j=m+1}^n \sum_{k=1}^m \left[ a_j \frac{\partial a_k}{\partial x_j} c_k + \frac{1}{2} \frac{\partial^2 a_k}{\partial x_j^2} c_k \right] $\\
$+ \frac{1}{\epsilon} \sum_{j=1}^m \sum_{k= m+1}^n \left[ a_j \frac{\partial a_k}{\partial x_j} c_k + \frac{1}{2} \frac{\partial^2 a_k}{\partial x_j^2} c_k \right] 
+ \frac{1}{\epsilon^2} \sum_{j=m+1}^n \sum_{k=m+1}^n \left[ a_j \frac{\partial a_k}{\partial x_j} c_k + \frac{1}{2} \frac{\partial^2 a_k}{\partial x_j^2} c_k \right]  $
\end{itemize}


Therefore, 
\begin{equation} 
\begin{aligned}
f( X_\tau) =& f(X_\rho) \\
& + \sum_{j=1}^n f_{(j)} (X_\rho) \int_\rho^\tau dW_s^j 
  + f_{(0)} (X_\rho) \int_\rho^\tau ds \\
& + \sum_{j=1}^n \int_\rho^\tau \int_\rho^{s_2} f_{(j,0)} (s_1) dW_{s_1}^j ds_2 \\
& + \int_\rho^\tau \int_\rho^{s_2} f_{(0,0)} (s_1) ds_1 ds_2 
\end{aligned}
\end{equation}

Up to order $\mathcal{O} ((\tau - \rho)^2)$, we have
\begin{equation}
\begin{aligned}
& f_1(X_\tau) f_2(X_\tau) = \\
f_1(X_\rho) 
& \left( f_2(X_\rho) 
 + \sum_{j=1}^n f_{2(j)} (X_\rho) \int_\rho^\tau dW_s^j 
 + f_{2(0)} (X_\rho) \int_\rho^\tau ds \right. \\
& \left. + \sum_{j=1}^n \int_\rho^\tau \int_\rho^{s_2} f_{2(j,0)} (s_1) dW_{s_1}^j ds_2 
 + \int_\rho^\tau \int_\rho^{s_2} f_{2(0,0)} (s_1) ds_1 ds_2 \right) \\
 + \left( \sum_{j=1}^n f_{1(j)}(X_\rho) \int_\rho^\tau dW_s^j \right)
& \left( f_2(X_\rho) 
 + \sum_{j=1}^n f_{2(j)} (X_\rho) \int_\rho^\tau dW_s^j 
 + f_{2(0)} (X_\rho) \int_\rho^\tau ds \right. \\
& \left. + \sum_{j=1}^n \int_\rho^\tau \int_\rho^{s_2} f_{2(j,0)} (s_1) dW_{s_1}^j ds_2 \right) \\
+ \left( f_{1(0)} (X_\rho) \int_\rho^\tau ds \right)
& \left( f_2(X_\rho) 
 + \sum_{j=1}^n f_{2(j)} (X_\rho) \int_\rho^\tau dW_s^j 
 + f_{2(0)} (X_\rho) \int_\rho^\tau ds \right) \\
 + \left( \sum_{j=1}^n \int_\rho^\tau \int_\rho^{s_2} f_{1(j,0)}(s_1) dW_{s_1}^j ds_2 \right)
& \left( f_2(X_\rho) 
 + \sum_{j=1}^n f_{2(j)} (X_\rho) \int_\rho^\tau dW_s^j  \right) \\
 + \left( \int_\rho^\tau \int_\rho^{s_2} f_{1(0,0)} (s_1) ds_! ds_2 \right)
& \left( f_2(X_\rho) \right)
\\ & + \mathcal{O} ((\tau - \rho)^{5/2})
\end{aligned}
\end{equation}

Therefore, we have
\begin{equation}
\begin{aligned}
& \mathbb{E} [f_1(X_\tau) f_2(X_\tau) ] = \\
\mathbb{E} \left[ \right.
& f_1(X_\rho) 
 \left( f_2(X_\rho) 
 + f_{2(0)} (X_\rho) (\tau - \rho) 
 + \sum_{j=1}^n  \int_\rho^\tau \int_\rho^{s_2} f_{2(j,0)} (s_1) dW_{s_1}^j ds_2 
 + \int_\rho^\tau \int_\rho^{s_2} f_{2(0,0)} (s_1) ds_1 ds_2 \right) \\
 & + \left( \sum_{j=1}^n f_{1(j)}(X_\rho) \int_\rho^\tau dW_s^j \right)
  \left( \sum_{j=1}^n f_{2(j)} (X_\rho) \int_\rho^\tau dW_s^j 
 + \sum_{j=1}^n \int_\rho^\tau \int_\rho^{s_2} f_{2(j,0)} (s_1) dW_{s_1}^j ds_2 \right) \\
& + \left( f_{1(0)} (X_\rho) (\tau - \rho) \right)
 \left( f_2(X_\rho) 
 + f_{2(0)} (X_\rho) (\tau - \rho) \right) \\
 & + \left( \sum_{j=1}^n \int_\rho^\tau \int_\rho^{s_2} f_{1(j,0)}(s_1) dW_{s_1}^j ds_2 \right)
\left( f_2(X_\rho) 
 + \sum_{j=1}^n f_{2(j)} (X_\rho) \int_\rho^\tau dW_s^j  \right) \\
 & + \left( \int_\rho^\tau \int_\rho^{s_2} f_{1(0,0)} (s_1) ds_! ds_2 \right)
 \left( f_2(X_\rho) \right) \left. \right]
\\ & + \mathcal{O} ((\tau - \rho)^{5/2})
\end{aligned}
\end{equation}

\begin{equation} 
\begin{aligned}
\mathbb{E} [f( X_\tau)] =& f(X_\rho) \\
& + f_{(0)} (X_\rho) (\tau - \rho) \\
& + \sum_{j=1}^n \mathbb{E} \left[ \int_\rho^\tau \int_\rho^{s_2} f_{(j,0)} (s_1) dW_{s_1}^j ds_2 \right] \\
& + \int_\rho^\tau \int_\rho^{s_2} f_{(0,0)} (s_1) ds_1 ds_2 
\end{aligned}
\end{equation}

\begin{equation}
\begin{aligned}
& \mathbb{E} [f_1(X_\tau) f_2(X_\tau) ] - \mathbb{E}[f_1(X_\tau)]\mathbb{E}[f_2(X_\tau)]= \\
\mathbb{E} \left[ \right.
& f_1(X_\rho) 
 \left( f_2(X_\rho) 
 + f_{2(0)} (X_\rho) (\tau - \rho) 
 + \sum_{j=1}^n  \int_\rho^\tau \int_\rho^{s_2} f_{2(j,0)} (s_1) dW_{s_1}^j ds_2 
 + \int_\rho^\tau \int_\rho^{s_2} f_{2(0,0)} (s_1) ds_1 ds_2 \right) \\
 & + \left( \sum_{j=1}^n f_{1(j)}(X_\rho) \int_\rho^\tau dW_s^j \right)
  \left( \sum_{j=1}^n f_{2(j)} (X_\rho) \int_\rho^\tau dW_s^j 
 + \sum_{j=1}^n \int_\rho^\tau \int_\rho^{s_2} f_{2(j,0)} (s_1) dW_{s_1}^j ds_2 \right) \\
& + \left( f_{1(0)} (X_\rho) (\tau - \rho) \right)
 \left( f_2(X_\rho) 
 + f_{2(0)} (X_\rho) (\tau - \rho) \right) \\
 & + \left( \sum_{j=1}^n \int_\rho^\tau \int_\rho^{s_2} f_{1(j,0)}(s_1) dW_{s_1}^j ds_2 \right)
\left( f_2(X_\rho) 
 + \sum_{j=1}^n f_{2(j)} (X_\rho) \int_\rho^\tau dW_s^j  \right) \\
 & + \left( \int_\rho^\tau \int_\rho^{s_2} f_{1(0,0)} (s_1) ds_! ds_2 \right)
 \left( f_2(X_\rho) \right) \left. \right] \\
 & - f_1(X_\rho) 
 \left( f_2(X_\rho) 
 + f_{2(0)} (X_\rho) (\tau - \rho) 
 + \sum_{j=1}^n  \mathbb{E} \left[ \int_\rho^\tau \int_\rho^{s_2} f_{2(j,0)} (s_1) dW_{s_1}^j ds_2  \right]
 + \int_\rho^\tau \int_\rho^{s_2} f_{2(0,0)} (s_1) ds_1 ds_2 \right)) \\
 & - f_{1(0)} (X_\rho)(\tau - \rho) \left( f_2(X_\rho) + f_{2(0)} (X_\rho) (\tau - \rho) \right) \\
 & - f_2(X_\rho) \left( \sum_{j=1}^n \mathbb{E} \left[ \int_\rho^\tau \int_\rho^{s_2} f_{1(j,0)} (s_1) dW_{s_1}^j ds_2 \right] 
 + \int_\rho^\tau \int_\rho^{s_2} f_{1(0,0)} (s_1) ds_1 ds_2 \right)
\\ & + \mathcal{O} ((\tau - \rho)^{5/2}) \\
= 
 & \left( \sum_{j=1}^n f_{1(j)}(X_\rho) \int_\rho^\tau dW_s^j \right)
  \left( \sum_{j=1}^n f_{2(j)} (X_\rho) \int_\rho^\tau dW_s^j 
 + \sum_{j=1}^n \int_\rho^\tau \int_\rho^{s_2} f_{2(j,0)} (s_1) dW_{s_1}^j ds_2 \right) \\
 & + \left( \sum_{j=1}^n \int_\rho^\tau \int_\rho^{s_2} f_{1(j,0)}(s_1) dW_{s_1}^j ds_2 \right)
\left(  \sum_{j=1}^n f_{2(j)} (X_\rho) \int_\rho^\tau dW_s^j  \right) \\
 & + \mathcal{O} ((\tau - \rho)^{5/2}) \\
 =  &  \sum_{j=1}^n \sum_{k=1}^n f_{1(j)}(X_\rho) f_{2(k)}(X_\rho) \mathbb{E} \left[ \left(\int_\rho^\tau dW_s^j \right)  \left(\int_\rho^\tau dW_s^k \right) \right] \\
 & + \sum_{j=1}^n \sum_{k=1}^n f_{1(j)}(X_\rho) \mathbb{E} \left[ \left(\int_\rho^\tau dW_s^j \right)  \left(\int_\rho^\tau \int_{\rho}^{s_2} f_{2(k,0)}(s_1) dW_{s_1}^k ds_2 \right) \right] \\ 
 & + \sum_{j=1}^n \sum_{k=1}^n f_{2(j)}(X_\rho) \mathbb{E} \left[ \left(\int_\rho^\tau dW_s^j \right)  \left(\int_\rho^\tau \int_{\rho}^{s_2} f_{1(k,0)}(s_1) dW_{s_1}^k ds_2 \right) \right] \\
& + \mathcal{O} ((\tau - \rho)^{5/2})
 \end{aligned}
\end{equation}


\end{document}